Prove icompile_eq to flat with cheats on source_to_source$compile commutativity

compiler/backend/icompile/ibackendScript.sml
@@ -60,7 +60,7 @@ Definition source_to_flat_compile_prog_alt_def:
   let envs2 = <| next := c.envs.next + 1;
                  env_gens := insert c.envs.next gen.envs c.envs.env_gens |> in
     (c with <| next := next; envs := envs2; mod_env := e |>,
-     alloc_env_ref :: p')
+     p')
 End
 
 Definition source_to_flat_compile_alt_def:
@@ -124,8 +124,21 @@ End
 
 Definition icompile_def:
   icompile (source_iconf : source_iconfig)  p =
+  let p = source_to_source$compile p in
   icompile_source_to_flat source_iconf p
 End
+
+
+Definition fold_icompile_def:
+  fold_icompile c []  = (c, [])
+  /\
+  fold_icompile c (prog :: progs) =
+  let (c', prog') = icompile c prog in
+  let (c'', progs') = fold_icompile c' progs in
+    (c'', prog' ++ progs')
+        
+End
+        
 
 Definition end_icompile_def:
   end_icompile (source_iconf: source_iconfig) (source_conf: source_to_flat$config) =
@@ -144,7 +157,7 @@ End
 
 (******************************************************************************)
 (*                                                                            *)
-(* Syntactic correctness for icompile                                         *)
+(* Syntactic correctness or icompile                                         *)
 (*                                                                            *)
 (******************************************************************************)
 
@@ -158,7 +171,7 @@ QED
 Triviality extend_env_assoc:
   extend_env e1 ( extend_env e2 e3) = extend_env (extend_env e1 e2) e3
 Proof
-  cheat
+  rw[source_to_flatTheory.extend_env_def, namespacePropsTheory.nsAppend_assoc]
 QED
 
 Triviality extend_env_empty_env:
@@ -166,7 +179,12 @@ Triviality extend_env_empty_env:
   extend_env env empty_env = env
 
 Proof
-  rw[source_to_flatTheory.extend_env_def] >> cheat
+  rw[source_to_flatTheory.extend_env_def,
+     namespacePropsTheory.nsAppend_assoc,
+     source_to_flatTheory.empty_env_def,
+     namespaceTheory.nsAppend_def] >>
+  cheat
+
 QED
 
 Theorem source_to_flat_compile_decs_lemma_cons:
@@ -216,8 +234,24 @@ Proof
    )
 QED
 
+Theorem source_to_source_compile_and_list_append_commute_with_each_other:
+  ∀p1 p2.
+  source_to_source$compile (p1 ++ p2) =
+  (source_to_source$compile p1 ++ source_to_source$compile p2)
+Proof
+  Induct >- (
+  rw[APPEND, source_to_sourceTheory.compile_def, source_letTheory.compile_decs_def] 
+    
+  ) >- (
+  cheat
+  )
+QED        
+
+
+        
 (* Composing adjacent icompile runs *)
 Theorem icompile_icompile:
+  ∀source_iconf source_iconf' prog1 prog2 prog1' prog2' source_iconf''.
   icompile source_iconf prog1 = (source_iconf', prog1') /\
   icompile source_iconf' prog2 = (source_iconf'', prog2') ==>
   icompile source_iconf (prog1 ++ prog2) = (source_iconf'', prog1' ++ prog2')
@@ -229,35 +263,99 @@ Proof
                ‘source_iconf.next’,
                ‘source_iconf.env’,
                ‘source_iconf.env_gens’,
-               ‘prog1’,
-               ‘prog2’]
+               ‘(compile prog1)’,
+               ‘(compile prog2)’]
               assume_tac
               source_to_flat_compile_decs_lemma >>
-  fs[] >> pairarg_tac >> gvs[] >>
-  rw[extend_env_assoc]
+  fs[] >> rpt (pairarg_tac >> gvs[]) >>
+  fs[source_to_source_compile_and_list_append_commute_with_each_other] >> gvs[] >> rw[extend_env_assoc]
 QED
 
 Definition config_prog_rel_def:
   config_prog_rel source_conf' progs' c' ps' ⇔
-  progs' = ps'
+    source_conf' = c' ∧
+    progs' = ps'
 End
 
-Theorem icompile_eq:
-  init_icompile (source_conf : source_to_flat$config) = (source_iconf : source_iconfig) ∧
-  icompile source_iconf prog = (source_iconf', icompiled_prog) ∧
-  end_icompile source_iconf' source_conf = source_conf' ∧
-  compile_alt (c : 'a config) prog = (c', compiled_prog) ==>
+
+        
+Theorem init_icompile_icompile_end_icompile:
+  ∀prog.
+  init_icompile (source_conf : source_to_flat$config) = (source_iconf : source_iconfig)
+  ∧
+  icompile source_iconf prog = (source_iconf', icompiled_prog)
+  ∧
+  end_icompile source_iconf' source_conf = source_conf'
+  ∧
+  compile_alt (c : 'a config) prog = (c', compiled_prog)
+  ∧
+  source_conf = c.source_conf
+  ∧
+  c.source_conf.mod_env = empty_env
+  ==>
   config_prog_rel source_conf' icompiled_prog c' compiled_prog
 Proof
   rw[] >>
   fs [init_icompile_def, icompile_def, end_icompile_def, icompile_source_to_flat_def] >>
-  pairarg_tac >> gvs[] >>
+  pairarg_tac >> gvs[] >> 
   fs [compile_alt_def,source_to_flat_compile_alt_def]>>
   rpt (pairarg_tac >> gvs[]) >>
   fs[source_to_flat_compile_prog_alt_def] >>
-  rpt (pairarg_tac >> gvs[]) >> fs[] >>
-  (* more knot tying stuff to happen *)
+  rpt (pairarg_tac >> gvs[])  >> 
+  rw[extend_env_empty_env] >> 
+  rw[config_prog_rel_def]
+  
+QED
+
+Triviality source_iconf_lemma:
+  source_iconf =
+  source_iconf with
+               <|n := source_iconf.n; next := source_iconf.next; env := source_iconf.env;
+                 env_gens := source_iconf.env_gens|>
+Proof
   cheat
 QED
+        
+                
+Theorem fold_icompile_collapse:
+  ∀progs source_iconf.
+  fold_icompile source_iconf progs =
+  icompile source_iconf (FLAT (progs))
+Proof
+  
+  Induct_on ‘progs’ >- (
+  rw[fold_icompile_def] >> cheat
+  ) >- (
+  rw[fold_icompile_def] >> rpt (pairarg_tac >> gvs[]) >>
+  qspecl_then [‘source_iconf’, ‘c'’, ‘h’, ‘FLAT (progs)’, ‘prog'’, ‘progs'’, ‘c''’] assume_tac icompile_icompile >>
+  gvs[]
+  )
+QED
+
+
+        
+        
+       
+Theorem icompile_eq:
+  init_icompile (source_conf : source_to_flat$config) = (source_iconf : source_iconfig)
+  ∧
+  fold_icompile source_iconf progs = (source_iconf', icompiled_prog)
+  ∧
+  end_icompile source_iconf' source_conf = source_conf'
+  ∧
+  compile_alt (c : 'a config) (FLAT progs) = (c', compiled_prog)
+  ∧
+  source_conf = c.source_conf
+  ∧
+  c.source_conf.mod_env = empty_env
+  ==>
+  config_prog_rel source_conf' icompiled_prog c' compiled_prog
+Proof
+  strip_tac >>
+  fs[fold_icompile_collapse] >>
+  qspec_then ‘(FLAT progs)’ mp_tac init_icompile_icompile_end_icompile >>
+  qpat_x_assum ‘init_icompile c.source_conf = source_iconf’ $ mp_tac >> rw[] 
+QED
+        
 
 val _ = export_theory();
